\mysection{Distributions}
\myssection{Binomial }

\mysssection{General}
$X$ = the number of successes in n trials.
This is n trials of a Bernoulli random variable.

\mysssection{Probability Mass Function}
$P\{X=k\} = \binom{n}{k}p^kq^{n-k}$, for $k=0,1,2,...,n,$ where $\binom{n}{k}=\frac{n!}{k!(n-k)!}$

\mysssection{Mean}
$m_x=np$

\mysssection{Variance}
$Var(x)=np(1-p)$
    
\myssection{Uniform }

\mysssection{General}
$X$ has equal likeliness of taking any value in the interval $[a,b]$

\mysssection{Probability Density Function}
$f_x(u) = \frac{1}{b-a}$, for $a<u<b$, and is 0 elsewhere

\mysssection{Cumulative Distribution Function}
\[ F_x(u)=
  \begin{cases} 
      0,               &     u < a \\
      \frac{u-a}{b-a}, & a < u < b \\
      1,               & b < u 
   \end{cases}
\]

\mysssection{Mean}
$m_x=(a+b)/2 $ 

\mysssection{Variance}
$Var(X)=\frac{(b-a)^2}{12}$
    

\myssection{Triangular }

\mysssection{General}
Upon adding two uniform distributions, we get the triangular density function. The function only has value over $[2a,2b]$

\mysssection{Density}
\[ f_x(\alpha)=
  \begin{cases} 
    \frac{\alpha-2a}{(b-a)^2}, & 2a<\alpha<(a+b) \\
    \frac{2b-\alpha}{(b-a)^2}, & (a+b)<\alpha<(2b) \\
    0,                         & otherwise
  \end{cases}
\]

\mysssection{Cumulative }
This was not listed in the summary, and I need to review to understand why.
    

\myssection{Exponential }

\mysssection{General}
$X$ is the time to arrival or time to failure, where arrival rate is $\lambda$ \\
$X$ can also be viewed as departure time with departure rate $\mu$

\mysssection{Probability Density Function}
$f_x(t) = \lambda e^{-\lambda t}$, for $t>0$, and is $0$ elsewhere.

\mysssection{Cumulative Distribution Function}
$F_x(t) = 1-e{-\lambda t}$, for $t\geq0$, and is $0$ elsewhere.

\mysssection{Mean and Variance}
$m_x=\sigma_x=1/\lambda$
    
\myssection{Gaussian }

\mysssection{General}
The normal distribution

\mysssection{Probability Density Function}
With mean $m$ and standard deviation $\sigma$ \\
$f_x(u)=\frac{1}{\sqrt{2\pi}\sigma}e^{-\frac{(u-m)^2}{2\sigma^2}}$ \\
Unit Gaussian (normal) $\sigma = 1$, $m=0$ \\
$f_x(u)=\frac{1}{\sqrt{2\pi}}e^{-\frac{u^2}{2}}$

\mysssection{Unit Gaussian Cumulative Distribution $\phi(u)$}
$\phi(u)$ was used to compute the following \\
$P\{a<X<b\}=\phi(\frac{b-m}{\sigma})-\phi(\frac{a-m}{\sigma})$

\mysssection{Mean and Variance}
$m$ and $\sigma$ are the mean and standard deviation \\
$\sigma_x^2$ is the variance
    

\myssection{Geometric }

\mysssection{General}
$X$ is the number of trials before the first success \\
$p$ is the probability of success

\mysssection{Mass Function}
$P\{X=k\} = p(1-p)^{k-1}$, for $k=1,2,3,...$

\mysssection{Mean}
$m_x=1/p$

\mysssection{Variance}
$Var(X)=(1-p)/p^2$

    

\myssection{Poisson }

\mysssection{General}
$X$ is the number of arrivals in a time interval $t$ \\
$\lambda$ is the arrival rate

\mysssection{Mass Function}
$P\{X=k\}=\frac{(\lambda t)^k}{k!}e^{\lambda t}$, for $k=0,1,2,3,...$

\mysssection{Mean and Variance}
$m_x= Var(X) = \lambda t$
    


